template-coq/theories/Constants.v
@@ -87,7 +87,6 @@ Register MetaCoq.Template.Universes.InProp as metacoq.ast.InProp.
 Register MetaCoq.Template.Universes.InSet as metacoq.ast.InSet.
 Register MetaCoq.Template.Universes.InType as metacoq.ast.InType.
 Register MetaCoq.Template.Universes.ConstraintType.Le as metacoq.ast.constraints.Le.
-Register MetaCoq.Template.Universes.ConstraintType.Lt as metacoq.ast.constraints.Lt.
 Register MetaCoq.Template.Universes.ConstraintType.Eq as metacoq.ast.constraints.Eq.
 Register MetaCoq.Template.Universes.Universe.from_kernel_repr as metacoq.ast.universe.from_kernel_repr.
 (* Register MetaCoq.Template.Universes.Universe.to_kernel_repr as metacoq.ast.universe.to_kernel_repr. *)
